inhtype.v
@@ -1,0 +1,100 @@
+From mathcomp Require Import ssreflect ssrfun ssrbool ssrnat seq fintype order.
+From mathcomp Require Import eqtype fingraph path. 
+From event_struct Require Import utilities.
+
+Set Implicit Arguments.
+Unset Strict Implicit.
+Unset Printing Implicit Defensive.
+
+Module Inhabitant.
+
+Section ClassDef.
+
+Record mixin_of T0 (b : Equality.class_of T0) (T := Equality.Pack b) :=
+  Mixin { inh : T }.
+
+Set Primitive Projections.
+Record class_of (T : Type) := Class {
+  base   : Equality.class_of T;
+  mixin  : mixin_of base;
+}.
+Unset Primitive Projections.
+
+Local Coercion base : class_of >-> Equality.class_of.
+
+Structure type := Pack { sort; _ : class_of sort }.
+
+Local Coercion sort : type >-> Sortclass.
+
+Variables (T : Type) (cT : type).
+
+Definition class := let: Pack _ c as cT' := cT return class_of cT' in c.
+Definition clone c of phant_id class c := @Pack T c.
+
+Definition pack :=
+  fun bT b & phant_id (Equality.class bT) b =>
+  fun m => Pack (@Class T b m).
+
+(* Inheritance *)
+Definition eqType := @Equality.Pack cT class.
+End ClassDef.
+
+Module Exports.
+Coercion base : class_of >-> Equality.class_of.
+Coercion sort : type >-> Sortclass.
+Coercion eqType : type >-> Equality.type.
+Canonical eqType.
+Notation inhType := type.
+Definition inh {T : inhType} : T := inh (mixin (class T)).
+Notation Inhabitant T m := (@pack T _ _ id m).
+Notation "[ 'inhType' 'of' T 'for' cT ]" := (@clone T cT _ id)
+  (at level 0, format "[ 'inhType'  'of'  T  'for'  cT ]") : form_scope.
+Notation "[ 'inhType' 'of' T ]" := [inhType of T for _]
+  (at level 0, format "[ 'inhType'  'of'  T ]") : form_scope.
+End Exports.
+
+End Inhabitant.
+Export Inhabitant.Exports.
+Implicit Type T : inhType.
+
+Section Extension.
+
+Context {T : inhType}.
+Implicit Types (x : T) (n : nat).
+Notation inh := (@inh T).
+
+Definition ext {n} (f : 'I_n -> T) : nat -> T := fun k =>
+  if insub_ord n k is some k then f k else inh.
+
+Lemma ext_add {x n} {f : 'I_n -> T} r : r != n ->
+  ext (add f x) r = ext f r.
+Proof.
+  rewrite /ext. insub_case=> ??; insub_case=> //; try slia.
+  move => L. rewrite add_lt. exact /congr1 /ord_inj.
+Qed.
+
+Lemma ext_add_n  {x n} {f : 'I_n -> T} :
+  ext (add f x) n = x.
+Proof. rewrite /ext. insub_case=> *; try slia. by rewrite add_ord_max. Qed.
+
+Lemma pred_ext {n} (f : 'I_n -> T) (p : pred T) (r : 'I_n) :
+ p (ext f r) = p (f r).
+Proof.
+  case: r=> /= *. rewrite /ext. insub_case=> [?|]; try slia.
+  exact /congr1 /congr1 /ord_inj.
+Qed.
+
+Lemma rel_ext {n x} (f : 'I_n -> T) (r : rel T) (a b : nat) :
+   ~ (rfield r inh) -> (r \o2 ext f) a b -> (r \o2 ext (add f x)) a b.
+Proof.
+  rewrite /comp2=> ?. case L: (a < n).
+  { rewrite ext_add //; try slia.
+    case L': (b < n). 
+    { rewrite ext_add //. slia. }
+    rewrite {2}/ext. insub_case=> [? _|_/(codom_rfield r)]; slia. }
+  rewrite {1}/ext. insub_case=> [? _|_/(dom_rfield r)]; slia.
+Qed.
+
+End Extension.
+
+
