regmachine.v
@@ -1,0 +1,112 @@
+From mathcomp Require Import ssreflect ssrfun ssrbool ssrnat seq fintype order.
+From mathcomp Require Import eqtype fingraph path finmap choice. 
+From event_struct Require Import utilities eventstructure inhtype.
+From event_struct Require Import transitionsystem.
+
+Set Implicit Arguments.
+Unset Strict Implicit.
+Unset Printing Implicit Defensive.
+
+Arguments Read {_ _}.
+Arguments Write {_ _}.
+
+Section RegMachine.
+
+Open Scope fmap.
+Context {val : inhType}.
+
+Notation n := (@n val).
+Notation exec_event_struct := (@exec_event_struct val).
+Notation lab := (@lab val).
+
+
+(* Registers --- thread local variables *)
+Definition reg := nat. 
+
+(* Instruction *)
+Inductive instr :=
+| WriteReg : val -> reg -> instr
+| ReadLoc  : reg -> loc -> instr
+| WriteLoc : val -> loc -> instr
+| CJmp     : reg -> nat -> instr.
+
+Definition seqprog := seq instr.
+
+Definition parprog := seq seqprog.
+
+Definition thrd_state := (nat * {fmap reg -> val})%type. 
+
+Variable p : seqprog.
+
+Notation nth := (nth (CJmp 0 0)).
+
+Definition thrd_sem (st : thrd_state) :
+  (option (@label unit val) * (val -> thrd_state))%type :=
+  let: (ip, map) := st in
+  match nth p ip with
+  | WriteReg v r => (none,             fun _ => (ip.+1, map.[r <- v]))
+  | ReadLoc  r x => (some (Read x tt), fun v => (ip.+1, map.[r <- v]))
+  | WriteLoc v x => (some (Write x v), fun _ => (ip.+1, map))
+  | CJmp     r n => (none,             fun _ => 
+                                             (if map.[? r] is some v then
+                                                if v == inh then ip.+1 else n
+                                              else ip.+1, map))
+  end.
+
+Definition ltr_thrd_sem (l : option (@label val val)) (st1 st2 : thrd_state) : bool :=
+  match thrd_sem st1, l with
+  | (some (Write x v), st), some (Write y u) => [&& x == y, v == u & st inh == st2]
+  | (some (Read  x _), st), some (Read  y u) => (x == y) && (st u == st2)
+  | (none            , st), none             => st inh == st2
+  | _, _                                     => false
+  end.
+
+Variable (es : exec_event_struct).
+
+Definition ocompatible (k : 'I_(n es)) (v : val) (x : loc) : 
+  {? k : 'I_(n es) |
+      compatible (ext (@lab es) k) (Read x v)} := 
+  insub k.
+
+Fixpoint compatible_seq_aux (x : loc) (k : nat) :
+  seq {v : val &
+      {k : 'I_(n es) |
+         compatible (ext (@lab es) k) (Read x v)}}
+ := 
+  if k is k'.+1 then
+    if insub k is some r then
+      if lab r is Write y v then
+        if x == y then
+          if ocompatible r v x is some comp then
+            (existT _ v comp) :: (compatible_seq_aux x k')
+          else compatible_seq_aux x k'
+        else compatible_seq_aux x k'
+      else compatible_seq_aux x k'
+    else [::]
+  else [::].
+
+Definition compatible_seq (x : loc) :
+  seq {v : val & {k : 'I_(n es) | compatible (ext (@lab es) k) (Read x v)}}
+  := compatible_seq_aux x (n es).-1.
+
+Fixpoint es_seq x op
+  (s : seq {v : val &
+           {k : 'I_(n es) |
+              compatible (ext (@lab es) k) (Read x v)}}) : 
+           seq (exec_event_struct * val) := 
+  if s is (existT v comp) :: st then
+      (add_event (Add op (fun=> comp)), v) :: 
+      es_seq op st
+  else [::].
+
+Definition add_label_unit_val 
+  (l : @label unit val) (op : option 'I_(n es)) :
+  seq (exec_event_struct * val) :=
+  match l with
+  | Read x tt   => es_seq op (compatible_seq x)
+  | Write x v   => [:: (add_event 
+      (@Add _ es (Write x v) op (fun x => match Bool.diff_false_true x with end)), v)]
+  | _          => [::]
+  end.
+
+End RegMachine.
